examples/isEven.v
@@ -1,0 +1,34 @@
+Require Export SystemFR.Notations.
+Require Export SystemFR.Evaluator.
+Require Extraction.
+Import Notations.UnTyped.
+
+
+Definition natEq_example := Eval compute in 
+  [|
+   let natEq := (
+         def_rec nat_eq x y =>
+         match x with
+         | 0 => match y with
+               | 0 => t_true
+               | s y' => t_false end
+         | s x' =>
+           match y with
+           | 0 =>  t_false
+           | s y' => (nat_eq x' y')
+           end
+         end) in
+   natEq 0 (s 0) |].
+
+
+Print natEq_example.
+
+
+Extraction Language Ocaml.
+Set Extraction AccessOpaque.
+
+Definition result := (eval natEq_example 1000).
+Extraction "isEven.ml" result. (* Fails with : Fetching opaque proofs from disk for SystemFR.Evaluator
+Error: The value you are asking for (getApp) is not available in this process. If you really need this, pass the
+"-async-proofs off" option to CoqIDE to disable asynchronous script processing and don't pass "-quick" to coqc *)
+
